Phi_Examples/Binary_Search.thy
@@ -2,6 +2,8 @@ theory Binary_Search
   imports Phi_Semantics.PhiSem_C
 begin
 
+(* ML \<open>PLPR_Statistics.reset_utilization_statistics_all ()\<close>  *)
+
 declare [[\<phi>LPR_collect_statistics program start,
           collecting_subgoal_statistics,
           recording_timing_of_semantic_operation,
@@ -73,5 +75,7 @@ text \<open>Semantic Representations of the Programs: \<close>
 
 thm binary_search_array_def
 thm generalized_binary_search_def
+
+ML \<open>report_utilization ["program"] [@{reasoner_group %all_derived_rules} ] \<close>
 
 end
