Phi_Examples/PhiEx_All.thy
@@ -22,6 +22,7 @@ ML \<open>
     | filter_out (Abs (_, _, X)) = filter_out X
     | filter_out (Const(\<^const_name>\<open>HOL.implies\<close>, _) $ _ $ X) = filter_out X
     | filter_out (Const(\<^const_name>\<open>Identifier_of\<close>, _) $ _ $ _ $ _) = true
+    | filter_out (Const(\<^const_name>\<open>Semantic_Type\<close>, _) $ _ $ _) = true
     | filter_out _ = false
 
   fun report_utilization statistic_groups reasoner_groups =
@@ -40,6 +41,27 @@ ML \<open>
                       ))]) reasoner_groups)) ]
       ) statistic_groups))
   end
+
+  fun report_utilization_to_file statistic_groups reasoner_groups =
+    let open File_Stream
+     in open_output (fn out =>
+        List.app (fn (column,sgroup) => (
+          output out column ; output out "\n" ;
+          List.app (fn (name, rgroup) => (
+            output out name ;
+            output out ", " ;
+            output out (string_of_int (
+              Phi_Reasoner.utilization_of_group_in_all_theories
+                (Context.Theory \<^theory>) (the (snd rgroup)) [sgroup]
+                  |> filter (fn (th, i) => i > 0 andalso
+                                not (filter_out (Thm.concl_of th)))
+                  |> length));
+            output out "\n"
+          )) reasoner_groups;
+          output out "\n"
+      )) statistic_groups
+    ) (Path.make ["Phi_Examples", "usage_of_generated_rules.csv"])
+    end
 
   val counters = [transformation_counter]
   fun report_transformation_performance () =
@@ -77,20 +99,29 @@ ML \<open>
 \<close>
 
 ML \<open>report_utilization ["program", "derivation"]
-       [ @{reasoner_group %Bin_Search_Tree} ] \<close>
-
-(*
-ML \<open>report_utilization ["program", "derivation"]
        [@{reasoner_group %Field}, @{reasoner_group %Array},
         @{reasoner_group %\<phi>MapAt}, @{reasoner_group %\<phi>MapAt_L}, @{reasoner_group %\<phi>Some},
         @{reasoner_group %Mem_Coercion}, @{reasoner_group %\<phi>Share},
         @{reasoner_group %Resource_Space},
         @{reasoner_group %Var}, @{reasoner_group %MemBlk},
-        @{reasoner_group %\<phi>Mul_Quant_Tree},
+        @{reasoner_group %\<phi>Mul_Quant_Tree}, @{reasoner_group %\<phi>Mul_Quant},
         @{reasoner_group %Linked_Lst}, @{reasoner_group %Dynamic_Array_arbi_len.DynArr},
         @{reasoner_group %BinTree}, @{reasoner_group %Bin_Search_Tree}, @{reasoner_group %AVL_Tree},
   @{reasoner_group %Hash} ] \<close>
-*)
+
+ML \<open>report_utilization_to_file [("column R", "program"), ("column R'", "derivation")]
+      [("Record", @{reasoner_group %\<phi>MapAt_L}),
+       ("Variable", @{reasoner_group %Var}),
+       ("Ref", @{reasoner_group %MemBlk}),
+       ("Quantifier Star", @{reasoner_group %\<phi>Mul_Quant}),
+       ("Array Slice", @{reasoner_group %\<phi>Mul_Quant_Tree}),
+       ("Linked List", @{reasoner_group %Linked_Lst}),
+       ("Dynamic Array", @{reasoner_group %Dynamic_Array_arbi_len.DynArr}),
+       ("Binary Tree", @{reasoner_group %BinTree}),
+       ("Search Tree", @{reasoner_group %Bin_Search_Tree}),
+       ("Lookup AVL", @{reasoner_group %AVL_Tree}),
+       ("Bucket Hash", @{reasoner_group %Hash})]  \<close>
+
 ML \<open>report_transformation_performance ()\<close>
 ML \<open>report_timing ()\<close>
 
