Phi_Logic_Programming_Reasoner/PLPR.thy
@@ -61,8 +61,6 @@ in fn thy => thy
                                         pretty_term_style
 end\<close>
 
-declare [[ML_debugger]]
-
 ML_file \<open>library/imporved_net.ML\<close>
 ML_file \<open>library/tools/ml_thms.ML\<close>
 ML_file \<open>library/pattern.ML\<close>
